\section{Proofs}
\lecture{02}{Aug 19 10:15}{Proofs}
\subsection{Deductive Reasoning}
\begin{definition*}[Deductive Reasoning]\label{def:deductive-reasoning}
    The process of making deductive arguments
\end{definition*}
\begin{definition*}[Deductive Argument]\label{def:deductive-argument}
    Process of making a logical inference
\end{definition*}
\begin{definition*}[Inference]\label{def:inference}
    Claim that a certain \hyperref[def:predicate]{predicate}, called the \textbf{conclusion}, follows from one or more \hyperref[def:predicate]{predicates}, called the \textbf{premises}.
\end{definition*}
Predicate $B$ \textbf{follows from} $A$ if it is impossible simultaneously for $A$ to be True and $B$ to be False

An inference is \textbf{valid} if the conclusion follows from the premises

A deductive argument is \textbf{sound} if the inference is valid and its premises are True

\subsection{More Logic Notation and Terminology}
\begin{definition*}[Universal Quantification Symbol ($\forall$)]\label{def:universal-quantification-symbol}
    Denotes that a proposition is True for all members
\end{definition*}
\begin{eg}
    \[
    \forall x \in \N:x^2 \geq x
    \]
    Read: ``\textbf{for all} (every, any, each) $x$ in \N\ the predicate ($x^2 \geq x$) evaluates to True''
\end{eg}
\begin{definition*}[Existential Quantification Symbol($\exists$)]\label{def:existential-quantification-symbol}
    Denotes that a proposition is True for at least one member
\end{definition*}
\begin{eg}
    \[
    \exists x \in \N:x^2<x
    \]
    Read: ``\textbf{there exists} an $x$ in \N\ such that the predicate $x^2<x$ evaluates to true''

    
\end{eg}
\begin{note}
        This is an example of a False proposition
\end{note}

\subsection{Contraposition}
\begin{definition*}[Contraposition]\label{def:contraposition}
    
    Let $p,q$ be predicates and consider the conditional statement
    \[
    p \implies q
    \]
    The \textbf{contrapositive} form of the statement is
    \[
    \neg q \implies \neg p
    \]

    A conditional statement and its contrapositive form are \textbf{equivalent}
    \[
    (p \implies q) \iff (\neg q \implies \neg p)
    \]
    When judging truthfulness of a statement, it sometimes helps to consider its contrapositive
\end{definition*}
Also existing, but not as common are:
\begin{itemize}
    \item The \textbf{inverse}: $\neg p \implies \neg q$
    \item The \textbf{converse}: $q \implies p$
    \item The \textbf{complement}: $\neg(p \implies q)$
\end{itemize}

\subsection{Proofs}

\begin{definition*}[Mathematical Proof]\label{def:proof}
    A deductive argument about something related to math. Uses spken/written language, or even sketches/diagrams.

    Usually rigorous (spells out assumptions and deductive steps as is convenient) but informal (some natural language with occasionally ambiguous symbols/rules) deductive reasoning
\end{definition*}
\begin{proposition}
    Let $n,m \in \N$ and suppose $n,m$ are even; then $(n+m)$ is even
\end{proposition}
\begin{proof}\ 
\begin{itemize}
    \item Since $n$ is even $\exists k \in \N$ such that $n=2k$
    \item Since $m$ is even $\exists q \in \N$ such that $n=2q$
    \item Then $(n+m)=(2k+2q)=2(k+q)$
    \item Therefore, $(n+m)$ is even
\end{itemize}
\begin{note}
    We used a method called \textbf{direct proof}
\end{note}
\end{proof}
\subsection{Mathematical Induction}
\begin{definition*}[Mathematical Induction]\label{def:mathematical-induction}
    If asked to prove that a certain proposition, $P(n)$ is true for any $n \in \N$, we will accept as proof the following inference, if sound:
    \begin{equation*}
        \begin{array}{c}
            P(1) = \text{T} \tag{1} \\
            \left(P(k) \stackrel{2}{=} \text{T}\right) \Rightarrow \left(P(k+1) = \text{T}\right)
        \end{array}
        \stackrel{3}{\Rightarrow} P(n) = \text{T}, \forall n \in \mathbb{N}
    \end{equation*}
    Where (1) is called the \textbf{base case}; (2) is called the \textbf{induction hypothesis}; (3) is the \textbf{induction step}
\end{definition*}
A variant called \textbf{complete} (or strong/generalized) induction uses a stronger hypothesis in the induction step:
\[
(P(j),\forall j \leq k) \implies P(k+1)
\]
\begin{proposition}
    For any $n \in \N$
    \[
    1+2+\cdots+n=\frac{n(n+1)}{2}
    \]
\end{proposition}
\begin{proof}
    By induction
    \begin{itemize}
        \item Base case: for $n=1$,$\frac{n(n+1)}{2}=1$
        \item Induction step: suppose, for some $k \in \N$, $1+2+\cdots+k=\frac{k(k+1)}{2}$, then
        \begin{align*}
        1+2+\cdots+k+(k+1)&=\frac{k(k+1)}{2}+(k+1) \\
        &=\frac{k(k+1)}{2}+\frac{2(k+1)}{2}=\frac{(k+1)(k+2)}{2}
        \end{align*}
    \end{itemize}
\end{proof}
\begin{proposition}
    Let $n \in \N$, if $n^2$ is even then $n$ is even
\end{proposition}
\begin{proof} By Contraposition \\
    Suppose $n$ were not even, then
    \begin{itemize}
        \item $n$ is odd, therefore
        \item $\exists k \in \N$ such that $n=2k-1$, and therefore
        \item $n^2=n\cdot n=(2k-1)(2k-1)=4k^2-4k+1=4(k^2-k)+1$
        \item Let $p=4(k^2-k)$, then
        \item $p\div2=2(k^2-k)$, therefore
        \item $p$ is even, therefore
        \item $n^2=p+1$ is odd
        \item Since $n^2$ is not odd, $n$ cannot be not even
    \end{itemize}
\end{proof}
\begin{proposition}
    $\sqrt{2}$ is irrational
\end{proposition}
\begin{proof}
    By contradiction \\
    Suppose $\sqrt{2}$ is rational, then
    \begin{itemize}
        \item $\exists p,q \in \N$ such that $\sqrt{2}=\frac{p}{q}$ and $p$ and $q$ have no common factors,
    \end{itemize}
\end{proof}
\subsection{Things that often need proving}
\begin{itemize}
    \item Existence: $\exists x \text{ such that } P(x)$ Proof by construction describes who the required $x$ is, and verifies $P(x)=\top$ (Don't need to actually find the thing)
    \item Uniqueness: $\left(P(x) \land P(y)\right) \implies (x=y)$ Name two things with the property and show they must be equal
\end{itemize}
\subsection{Proof of Equivalence}
To prove $P \iff Q$, prove both $P \implies Q$ and $Q \implies P$
Related: show two sets $A,B$ are equal by showing $A \subseteq B$ and $B \subseteq A$
To prove the following are equivalent (TFAE) you could prove a circular chain of implications
\[
\left(A \implies B\right) \land \left(B \implies C\right) \land \left(C \implies D\right) \land \left(D \implies A\right)
\]
